modified:   assembly/64bits/register.asm 	modified:   assembly/64bits/register.s 	modified:   assembly/64bits/test.sh 	modified:   assembly/hacking/clean.sh 	modified:   assembly/hacking/hacking.c 	modified:   assembly/hacking/hacking.h 	new file:   assembly/hacking/simple_server.c 	modified:   c/macro.c 	modified:   clean.sh 	deleted:    coq/README 	modified:   coq/le.v 	modified:   coq/logic.v 	copied:     coq/logic.v -> coq/logic2.v 	new file:   scheme/clean.sh 	modified:   scheme/evaluator/TODO 	modified:   scheme/evaluator/application.scm 	modified:   scheme/evaluator/test.scm 	modified:   scheme/evaluator/unit-test.scm 	new file:   scheme/main.c 	new file:   scheme/main.scm 	new file:   scheme/simple-guile.c

assembly/64bits/register.asm
@@ -13,22 +13,7 @@ text1   db      "register.asm is running ...", 0x0a
 
 _start:
         ; 256 bits
-        vmovupd  ymm0, [g_256]
-        vmovupd  ymm1, [g_256]
-        vmovupd  ymm2, [g_256]
-        vmovupd  ymm3, [g_256]
-        vmovupd  ymm4, [g_256]
-        vmovupd  ymm5, [g_256]
-        vmovupd  ymm6, [g_256]
-        vmovupd  ymm7, [g_256]
-        vmovupd  ymm8, [g_256]
-        vmovupd  ymm9, [g_256]
-        vmovupd  ymm10,[g_256]
-        vmovupd  ymm11,[g_256]
-        vmovupd  ymm12,[g_256]
-        vmovupd  ymm13,[g_256]
-        vmovupd  ymm14,[g_256]
-        vmovupd  ymm15,[g_256]
+;        vmovupd  ymm0, [g_256]
         
 
         ; 128 bits
