assembly/hacking/hacking.c
@@ -20,3 +20,26 @@ void *ec_malloc(unsigned int size) {
   return ptr;
 }
 
+// Dumps raw memory in hex byte and printable split format
+void dump(const unsigned char *data_buffer, unsigned int length) {
+  unsigned char byte;
+  unsigned int i, j;
+  for(i=0; i < length; i++) {
+    byte = data_buffer[i];
+    printf("%02x ", data_buffer[i]); // Display byte in hex.
+    if(((i%16)==15) || (i==length-1)) {
+      for(j=0; j < 15-(i%16); j++)
+        printf(" ");
+      printf("| ");
+      for(j=(i-(i%16)); j <= i; j++) { // Display printable bytes from line.
+        byte = data_buffer[j];
+        if((byte > 31) && (byte < 127)) // Inside printable char range
+          printf("%c", byte);
+        else
+          printf(".");
+        }
+      printf("\n"); // End of the dump line (each line is 16 bytes)
+    } // End if
+  } // End for
+}
+
