c/macro.c
@@ -1,19 +1,40 @@
-#include<stdio.h>
-//#include<string.h>
-//#include<malloc.h>
-//#include<assert.h>
+#include <stdio.h>
+
+// #EXP is stringification of argument
+
+#define WARN_IF(EXP) \
+  do { if(EXP) \
+          fprintf(stderr, "Warning: " #EXP "\n"); } \
+  while(0)
+
+// ok but syntactically odd (missing ';')
+#define WARN_IF_AGAIN(EXP) \
+  if(EXP) \
+    fprintf(stderr, "Warning again: " #EXP "\n")
+
+// ok but usage is odd
+#define WARN_IF_YET_AGAIN(EXP) \
+  if(EXP) \
+    fprintf(stderr, "Warning yet again: " #EXP "\n");
+
 
 
 int main()
 {
+  int i = 0;
+  int j = 1;
 
-//  using namespace std;
+  WARN_IF(i == 0);
+  WARN_IF(j == 0);
+  
+  WARN_IF_AGAIN(i == 0);
+  WARN_IF_AGAIN(j == 0);
 
-  printf("%s\n",__TIMESTAMP__);
+
+  WARN_IF_YET_AGAIN(i == 0) // odd syntax
+  WARN_IF_YET_AGAIN(j == 0) // odd syntax
 
   return 0;
-
-
 }
 
 
