scheme/evaluator/test.scm
@@ -1,12 +1,11 @@
 (load "main.scm")
 
-(lazy-eval '(define (try a b) (if (= 0 a) 1 b)))
-(lazy-eval '(define (test) (display "+++test is running+++") 2))
 
-
-;(lazy-eval '(try 0 (test)))
-
-(display (lazy-eval '(test)))(newline)
+(force-thunk 
+  (lazy-eval 
+    '(begin
+       (display "abcdef\n")
+       (display "+++test.scm is running+++\n"))))
 
 
 (exit 0)
