scheme/main.c
@@ -1,0 +1,14 @@
+#include <stdio.h>
+#include <stdlib.h>
+
+int main(){
+
+  char *s = getenv("HOSTNAME");
+
+  if(s == NULL)
+    printf("s is NULL\n");
+  else
+    printf("%s\n", getenv("HOSTNAME"));
+
+  return 0;
+}
