scheme/main.scm
@@ -1,0 +1,3 @@
+(display "+++main.scm is running+++")(newline)
+
+(exit 0)
