scheme/simple-guile.c
@@ -1,0 +1,31 @@
+// gcc -o simple-guile simple-guile.c $(pkg-config --cflags --libs guile-2.0)
+// For some reason, HOSTNAME needs to be exported first for my-hostname to work
+
+#include <stdlib.h>
+#include <libguile.h>
+
+static SCM
+my_hostname (void)
+{
+  char *s = getenv ("HOSTNAME");
+  if (s == NULL)
+    return SCM_BOOL_F;
+  else
+    return scm_from_locale_string (s);
+}
+
+static void
+inner_main (void *data, int argc, char **argv)
+{
+  scm_c_define_gsubr ("my-hostname", 0, 0, 0, my_hostname);
+  scm_shell (argc, argv);
+}
+
+int
+main (int argc, char **argv)
+{
+  scm_boot_guile (argc, argv, inner_main, 0);
+  return 0; /* never reached */
+}
+
+
