assembly/hacking/clean.sh
@@ -13,4 +13,5 @@ rm -f notesearch
 rm -f notetaker
 rm -f shellcode
 
+
 cd ${DIR}
