scheme/clean.sh
@@ -1,0 +1,10 @@
+#!/bin/sh
+
+DIR=`pwd`
+HOME=/home/john/Prog/scheme
+cd ${HOME}
+
+rm -f a.out
+rm -f *.o
+
+cd ${DIR}
